---
title: "Derive Black-Scholes Model"
---

In this page we derive the famous Black-Scholes Model for European option pricing.

<div style="background-color:white;color:blue;matrixOperation:20px;">
<ins>
### Geometric Brownian Motion
</ins>
</div>

Assuming the stock price follows geometric brownian motion and the SDE is:
$$dS_t = \mu S_t dt + \sigma S_t dW_t$$
and $g(x) = ln(x)$
Apply the Ito's formula:

$$
\begin{aligned}
dg(S_t) &= d(ln(S_t)) \\
&= \frac{1}{S_t}dS_t + \frac{1}{2} \cdot (-1) \cdot \frac{1}{S_t^2} \sigma^2 S_t^2dt \\
&= \frac{1}{S_t}(\mu S_t dt + \sigma S_t dW_t) - \frac{1}{2} \sigma^2dt \\
&= (\mu-\frac{1}{2} \sigma^2) dt + \sigma dW_t
\end{aligned}
$$
Take the integral, then we get the stock price $S_t$ at time $t$:

$$S_t = S_0 \cdot e^{(\mu-\frac{1}{2} \sigma^2) t + \sigma W_t}$$

**Expected value of $S_t$**: 

$$
\begin{aligned}
E[S_t] &= S_0 \cdot e^{(\mu-\frac{1}{2} \sigma^2) t } \cdot E[e^{\sigma W_t}] \\
&= S_0 \cdot e^{(\mu-\frac{1}{2} \sigma^2) t} \cdot e^{\frac{\sigma^2 t}{2}} \\
&= S_0 \cdot e^{(\mu-\frac{1}{2} \sigma^2) t+\frac{1}{2}\sigma^2 t} \\
&= S_0 \cdot e^{\mu t} \\
\end{aligned}
$$
We haven't proved that $E[e^{\sigma W_t}] = e^{\frac{1}{2}\sigma^2t}$ yet. Let's derive $E[e^{W_t}] = e^{\frac{1}{2}t}$ fisrt:

$$
\begin{aligned}
E[e^{W_t}] &= \int e^x \cdot \frac{1}{\sigma_w\sqrt{2\pi}} \cdot e^{-\frac{1}{2}(\frac{x-\mu}{\sigma_w})^2} dx\\
&= \int \frac{1}{\sqrt{t}\sqrt{2\pi}} \cdot e^{x-\frac{1}{2}(\frac{x}{\sqrt{t}})^2} dx \\
&= \int \frac{1}{\sqrt{t}\sqrt{2\pi}} \cdot e^{-x-\frac{x^2}{2t}} dx\\
&= \int \frac{1}{\sqrt{t}\sqrt{2\pi}} \cdot e^{-\frac{2xt+x^2}{2t}} dx\\
&= \int \frac{1}{\sqrt{t}\sqrt{2\pi}} \cdot e^{-\frac{x^2+2xt+t^2}{2t}+\frac{t^2}{2t}} dx\\
&= \int \frac{1}{\sqrt{t}\sqrt{2\pi}} \cdot e^{-\frac{1}{2}(\frac{x-(-t)}{\sqrt{t}})^2+\frac{t}{2}}  dx \\
&= e^{\frac{t}{2}} \cdot \int \frac{1}{\sqrt{t}\sqrt{2\pi}} \cdot e^{-\frac{1}{2}(\frac{x-(-t)}{\sqrt{t}})^2} dx  \\
&= e^{\frac{t}{2}} \\
\end{aligned}
$$
We can then extend to that $E[e^{\sigma W_t}] = e^{\frac{\sigma^2 t}{2}}$ by replacing $\sigma_w = \sqrt{t}$ with $\sigma_w = \sigma \sqrt{t}$


Geometric Brownian Motion means that the log of stock return follows normal distribution.





<div style="background-color:white;color:blue;matrixOperation:20px;">
<ins>
### Risk Neutral Measure & Girsanov's Theorem
</ins>
</div>




$$
\begin{aligned}
C &= E_Q[e^{-rT}(S_T-K)^+] \\
&= E_Q[e^{-rT}S_T \cdot I_{\{S_T-K\}}] - E_Q[e^{-rT}K \cdot I_{\{S_T-K\}}] \\
&= \text{1st term} - \text{2nd term}
\end{aligned}
$$

We will tackle the 1st term and 2nd term individually.

<div style="background-color:white;color:blue;matrixOperation:20px;">
<ins>
### The 1st Term
</ins>
</div>

$$
\begin{aligned}
E^Q[e^{-rT}S_T \cdot I_{\{S_T-K\}}] &= E^Q[e^{-rT}S_0 \cdot e^{(r-\frac{1}{2}\sigma^2)T+\sigma W_T^Q}\cdot I_{\{S_T-K\}}]\\
&= S_0 \cdot E_Q[e^{-\frac{1}{2}\sigma T+\sigma W_T^Q} I_{\{S_T-K\}}]\\
\end{aligned}
$$
Now we have to change the measure again using the Girsanov's Theorem . Define:

$$\frac{dQ^s}{dQ} = Z_t = e^{-\frac{1}{2}\sigma T+\sigma W_T^Q}$$
Then we can continue as 
$$
\begin{aligned}
S_0 \cdot E^Q[e^{-\frac{1}{2}\sigma T+\sigma W_T} I_{\{S_T-K\}}] &= S_0 \cdot E^Q[\frac{dQ^s}{dQ} \cdot  I_{\{S_T-K\}}]\\
&= S_0 \cdot E^{Q^s}[I_{\{S_T-K\}}] \\
&= S_0 \cdot Q^s[S_T>K] \\
&= S_0 \cdot Q^s[S_0 \cdot e^{(r-\frac{1}{2}\sigma^2)T+\sigma W_T^Q}>K] \\
&= S_0 \cdot Q^s[S_0 \cdot e^{(r-\frac{1}{2}\sigma^2)T+\sigma(W_T^{Q^s}+\sigma T)}>K] \\
&= S_0 \cdot Q^s[S_0 \cdot e^{(r+\frac{1}{2}\sigma^2)T+\sigma W_T^{Q^s}}>K] \\
&= S_0 \cdot Q^s[W_T^{Q^s}> \frac{ln(K/S_0)-(r+\frac{1}{2}\sigma^2)T}{\sigma}] \\
&= S_0 \cdot Q^s[\epsilon<\frac{ln(S_0/K)+(r+\frac{1}{2}\sigma^2)T}{\sigma \sqrt{T}}] \\
&= S_0 \cdot \Phi(d_1)
\end{aligned}
$$

Where 

$$d_1 = \frac{ln(S_0/K)+(r+\frac{1}{2}\sigma^2)T}{\sigma \sqrt{T}}$$

<div style="background-color:white;color:blue;matrixOperation:20px;">
<ins>
### The 2nd Term
</ins>
</div>

THe derivation of the 2nd term is always under $Q$ measure. i.e. $E[x] = E^Q[x]$ and $W_T = W^Q_T$

$$
\begin{aligned}
E[e^{-rT}K \cdot I_{\{S_T-K\}}] &= e^{-rT} \cdot K \cdot Q[S_T>K]\\
&= e^{-rT} \cdot Q[S_0 \cdot e^{(r-\frac{1}{2}\sigma^2)T + \sigma W_T}>K] \\
&= e^{-rT} \cdot Q[\epsilon>\frac{ln(K/S_0)-(r-\frac{1}{2}\sigma^2)T}{\sigma \sqrt{T}}] \\
&=  e^{-rT} \cdot Q[\epsilon<\frac{ln(S_0/K)+(r-\frac{1}{2}\sigma^2)T}{\sigma \sqrt{T}}] \\
&= e^{-rT} \cdot K \cdot \Phi(d_2)
\end{aligned}
$$

Where 
$$d_2 = \frac{ln(S_0/K)+(r-\frac{1}{2}\sigma^2)T}{\sigma \sqrt{T}}$$

